Use => via type_synonym

Launchbury/Env.thy
@@ -6,61 +6,54 @@ default_sort type
 
 subsubsection {* The type of finite maps *}
 
-typedef ('a, 'b) fmap  (infixr "f\<rightharpoonup>" 1) = "{x :: 'a \<Rightarrow> 'b. True }" by auto
+type_synonym  ('a, 'b) fmap = "'a \<Rightarrow> 'b" (infixr "f\<rightharpoonup>" 1)
 
-setup_lifting type_definition_fmap
+definition fdom :: "'key f\<rightharpoonup> 'value::pcpo \<Rightarrow> 'key set" where "fdom m = {x. m x \<noteq> \<bottom>}"
 
-lift_definition fdom :: "'key f\<rightharpoonup> 'value::pcpo \<Rightarrow> 'key set" is "\<lambda> m . {x. m x \<noteq> \<bottom>}" ..
+definition lookup :: "'key f\<rightharpoonup> 'value \<Rightarrow> 'key \<Rightarrow> 'value" (infix "f!" 55) where "lookup m x = m x"
 
-lift_definition lookup :: "'key f\<rightharpoonup> 'value \<Rightarrow> 'key \<Rightarrow> 'value" (infix "f!" 55) is "(\<lambda> x. x)" ..
+lemma lookup_fempty[simp]: "lookup \<bottom> x = \<bottom>" by (simp add: lookup_def)
 
-lift_definition fempty :: "'key f\<rightharpoonup> 'value::pcpo" ("f\<emptyset>") is "\<lambda> x. \<bottom>" by simp
+lemma fempty_fdom[simp]: "fdom \<bottom> = {}" by (simp add: fdom_def)
 
-lemma lookup_fempty[simp]: "lookup f\<emptyset> x = \<bottom>"
-  by transfer simp
+lemma fempty_fdom2[simp]: "fdom (\<lambda>_ . \<bottom>) = {}" by (simp add: fdom_def)
 
-lemma fempty_fdom[simp]: "fdom f\<emptyset> = {}"
-  by (transfer, auto)
+lemma fdomIff: "(a \<in> fdom m) = (lookup m a \<noteq> \<bottom>)" by (simp add: fdom_def lookup_def)
 
-lemma fdomIff: "(a : fdom m) = (lookup m a \<noteq> \<bottom>)"
- by (transfer, auto)
+lemma lookup_not_fdom: "x \<notin> fdom m \<Longrightarrow> lookup m x = \<bottom>"  by (auto iff:fdomIff)
 
-lemma lookup_not_fdom: "x \<notin> fdom m \<Longrightarrow> lookup m x = \<bottom>"
-  by (auto iff:fdomIff)
+lemma lookup_fdom[simp]: "m f! x \<noteq> \<bottom> \<Longrightarrow> x \<in> fdom m"  by (auto iff:fdomIff)
 
-lemma lookup_fdom[simp]: "lookup m x \<noteq> \<bottom> \<Longrightarrow> x \<in> fdom m"
-  by (auto iff:fdomIff)
-
-lemma fmap_eqI[intro]:
+lemma fmap_eqI:
   assumes "\<And> x. a f! x = b f! x"
   shows "a = b"
 using assms
-by(transfer) auto
+by (auto simp add: lookup_def)
 
 subsubsection {* Updates *}
 
-lift_definition
+definition
   fmap_upd :: "'key f\<rightharpoonup> 'value \<Rightarrow> 'key \<Rightarrow> 'value \<Rightarrow> 'key f\<rightharpoonup> 'value" ("_'(_ f\<mapsto> _')" [900,900]900)
-  is "\<lambda> m x v. m( x :=  v)"  by simp
+  where "fmap_upd m x v = m( x :=  v)"
 
 
 lemma fdom_fmap_upd_subset: "fdom (h (x f\<mapsto> v)) \<subseteq> insert x (fdom h)"
-  by (transfer, auto)
+  by (auto simp add: fdom_def fmap_upd_def)
 
 lemma lookup_fmap_upd[simp]: "lookup (h (x f\<mapsto> v)) x = v"
-  by (transfer, auto)
+  by (auto simp add: fdom_def fmap_upd_def lookup_def)
 
 lemma lookup_fmap_upd_other[simp]: "x' \<noteq> x \<Longrightarrow> lookup (h (x f\<mapsto> v)) x' = lookup h x'"
-  by (transfer, auto)
+  by (auto simp add: fdom_def fmap_upd_def lookup_def)
 
 lemma lookup_fmap_upd_eq: "lookup (h (x f\<mapsto> v)) x' = (if x = x' then v else lookup h x')"
-  by (transfer, auto)
+  by (auto simp add: fdom_def fmap_upd_def lookup_def)
 
 lemma fmap_upd_overwrite[simp]: "f (x f\<mapsto> y) (x f\<mapsto> z) = f (x f\<mapsto> z)"
-  by (transfer, auto) 
+  by (auto simp add: fdom_def fmap_upd_def lookup_def)
 
 lemma fmap_upd_noop[simp]: "x \<in> fdom f \<Longrightarrow> y = f f! x \<Longrightarrow> f (x f\<mapsto> y) = f"
-  by (transfer, auto)
+  by (auto simp add: fdom_def fmap_upd_def lookup_def)
 
 lemma fmap_upd_twist: "a \<noteq> c \<Longrightarrow> (m(a f\<mapsto> b))(c f\<mapsto> d) = (m(c f\<mapsto> d))(a f\<mapsto> b)"
   apply (rule fmap_eqI)
@@ -69,32 +62,27 @@ lemma fmap_upd_twist: "a \<noteq> c \<Longrightarrow> (m(a f\<mapsto> b))(c f\<m
   done
 
 lemma fmap_upd_eqD1: "m(a f\<mapsto> x) = n(a f\<mapsto> y) \<Longrightarrow> x = y"
-  by transfer (metis fun_upd_same)
+  by (metis fmap_upd_def fun_upd_same)
 
 subsubsection {* Restriction *}
 
-lift_definition fmap_restr :: "'a set \<Rightarrow> 'a f\<rightharpoonup> 'b::pcpo \<Rightarrow> 'a f\<rightharpoonup> 'b"
-  is "\<lambda> S m x. if x \<in> S then m x else \<bottom>"..
+definition fmap_restr :: "'a set \<Rightarrow> 'a f\<rightharpoonup> 'b::pcpo \<Rightarrow> 'a f\<rightharpoonup> 'b"
+  where "fmap_restr S m = (\<lambda> x. if x \<in> S then m x else \<bottom>)"
 
 abbreviation fmap_restr_rev  (infixl "f|`"  110) where "fmap_restr_rev m S \<equiv> fmap_restr S m"
 
-lemma fmap_restr_empty[simp]: "fdom m \<inter> S = {} \<Longrightarrow> m f|` S = f\<emptyset>"
-  apply transfer
-  by (metis (lifting, full_types) Int_Collect empty_iff inf_commute)
+lemma fmap_restr_empty[simp]: "fdom m \<inter> S = {} \<Longrightarrow> m f|` S = \<bottom>"
+  by (fastforce simp add: fdom_def fmap_restr_def)
 
 lemma lookup_fmap_restr[simp]: "x \<in> S \<Longrightarrow> lookup (fmap_restr S m) x = lookup m x"
-  by (transfer, auto)
+  by (fastforce simp add: fmap_restr_def lookup_def)
 
 lemma lookup_fmap_restr_not_there[simp]: "x \<notin> S \<Longrightarrow> lookup (fmap_restr S m) x = \<bottom>"
-  by (transfer, auto)
+  by (fastforce simp add: fmap_restr_def lookup_def)
 
 lemma lookup_fmap_restr_eq: "m f|` S f! x = (if x \<in> S then m f! x else \<bottom>)"
-  by (transfer, auto)
+  by (simp)
 
-(*
-lemma fdom_fmap_restr[simp]: "fdom (fmap_restr S m) = fdom m \<inter> S"
-  by (transfer, simp)
-*)
 
 lemma fmap_restr_cong: "fdom m \<inter> S1 = fdom m \<inter> S2 \<Longrightarrow> m f|` S1 = m f|` S2"
   apply (rule fmap_eqI)
@@ -103,7 +91,7 @@ lemma fmap_restr_cong: "fdom m \<inter> S1 = fdom m \<inter> S2 \<Longrightarrow
 
 lemma fmap_restr_fmap_restr[simp]:
  "x f|` d2 f|` d1 = x f|` (d1 \<inter> d2)"
- by (transfer, auto simp add: restrict_map_def)
+  by (fastforce simp add: fmap_restr_def lookup_def)
 
 lemma fmap_restr_fmap_restr_subset:
  "d1 \<subseteq> d2 \<Longrightarrow> x f|` d2 f|` d1 = x f|` d1"
@@ -129,42 +117,42 @@ lemma fmap_restr_fmap_upd_other[simp]: "x \<notin> S \<Longrightarrow> m1(x f\<m
 
 subsubsection {* Deleting *}
 
-lift_definition fmap_delete :: "'a \<Rightarrow> 'a f\<rightharpoonup> 'b \<Rightarrow> 'a f\<rightharpoonup> 'b::pcpo"
-  is "\<lambda> x m. m(x := \<bottom>)"..
+definition fmap_delete :: "'a \<Rightarrow> 'a f\<rightharpoonup> 'b \<Rightarrow> 'a f\<rightharpoonup> 'b::pcpo"
+  where "fmap_delete x m = m(x := \<bottom>)"
 
 lemma lookup_fmap_delete[simp]:
   "x' \<noteq> x \<Longrightarrow> fmap_delete x m f! x' = m f! x'"
-  by (transfer, simp)
+  by (simp add: fmap_delete_def lookup_def)
 
 lemma lookup_fmap_delete_None[simp]:
   "fmap_delete x m f! x = \<bottom>"
-  by (transfer, simp)
+  by (simp add: fmap_delete_def lookup_def)
 
 lemma fdom_fmap_delete[simp]:
   "fdom (fmap_delete x m) = fdom m - {x}"
-  by (transfer, auto)
+  by (auto simp add: fmap_delete_def lookup_def fdom_def)
 
 lemma fdom_fmap_delete_subset:
   "fdom (fmap_delete x m) \<subseteq> fdom m" by auto
 
 lemma fmap_delete_fmap_upd[simp]:
   "fmap_delete x (m(x f\<mapsto> v)) = fmap_delete x m"
-  by (transfer, simp)
+  by (auto simp add: fmap_delete_def fmap_upd_def)
 
 lemma fmap_delete_fmap_upd2[simp]:
   "(fmap_delete x m)(x f\<mapsto> v) = m(x f\<mapsto> v)"
-  by (transfer, simp)
+  by (auto simp add: fmap_delete_def fmap_upd_def)
 
 lemma fmap_delete_fmap_upd3[simp]:
   "x \<noteq> y \<Longrightarrow> fmap_delete x (m(y f\<mapsto> v)) = (fmap_delete x m)(y f\<mapsto> v)"
-  by (transfer, auto)
+  by (auto simp add: fmap_delete_def fmap_upd_def)
 
 lemma fmap_delete_noop[simp]:
   "x \<notin> fdom m \<Longrightarrow> fmap_delete x m = m"
-  by (transfer, auto)
+  by (auto simp add: fmap_delete_def fdom_def)
 
 lemma fmap_upd_fmap_delete[simp]: "x \<in> fdom \<Gamma> \<Longrightarrow> (fmap_delete x \<Gamma>)(x f\<mapsto> \<Gamma> f! x) = \<Gamma>"
-  by (transfer, auto)
+  by (auto)
 
 lemma fmap_restr_fmap_delete_other[simp]: "x \<notin> S \<Longrightarrow> fmap_delete x m f|` S = m f|` S"
   apply (rule fmap_eqI)
@@ -172,67 +160,48 @@ lemma fmap_restr_fmap_delete_other[simp]: "x \<notin> S \<Longrightarrow> fmap_d
   by (metis lookup_fmap_delete)
 
 lemma fmap_delete_restr: "fmap_delete x m = m f|` (-{x})"
-  by (auto simp add: lookup_fmap_restr_eq)
+  by (auto intro: fmap_eqI simp add: lookup_fmap_restr_eq)
 
 subsubsection {* Addition (merging) of finite maps *}
 
-lift_definition fmap_add :: "'a set \<Rightarrow> 'a f\<rightharpoonup> 'b \<Rightarrow> 'a f\<rightharpoonup> 'b \<Rightarrow> 'a f\<rightharpoonup> 'b"  
-  is "\<lambda> S f1 f2 x. if x \<in> S then f2 x else f1 x"..
+definition fmap_add :: "'a set \<Rightarrow> 'a f\<rightharpoonup> 'b \<Rightarrow> 'a f\<rightharpoonup> 'b \<Rightarrow> 'a f\<rightharpoonup> 'b"  
+  where "fmap_add S f1 f2 = (\<lambda> x. if x \<in> S then f2 x else f1 x)"
 
 abbreviation fmap_add_syn ("_ f++\<^bsub>_\<^esub> _" [100, 0, 100] 100) where "f1 f++\<^bsub>S\<^esub> f2 \<equiv> fmap_add S f1 f2"
 
-lemma fmap_add_fempty[simp]: "f\<emptyset> f++\<^bsub>S\<^esub> m = m f|` S" 
-  by (transfer, simp)
+lemma fmap_add_fempty[simp]: "\<bottom> f++\<^bsub>S\<^esub> m = m f|` S" 
+  by (auto simp add: fmap_add_def lookup_def fmap_restr_def)
 
-lemma fmap_add_fempty2[simp]: "m f++\<^bsub>S\<^esub> f\<emptyset>= m f|` (-S)" 
-  by (transfer, auto)
+lemma fmap_add_fempty2[simp]: "m f++\<^bsub>S\<^esub> \<bottom> = m f|` (-S)" 
+  by (auto simp add: fmap_add_def lookup_def fmap_restr_def)
 
 lemma fdom_fmap_add[simp]: "fdom (m1 f++\<^bsub>S\<^esub> m2) = (fdom m1 - S) \<union> (fdom m2 \<inter> S)"
-  by transfer auto
+  by (auto simp add: fmap_add_def lookup_def fdom_def)
 
 lemma lookup_fmap_add1[simp]: "x \<in> S \<Longrightarrow> m1 f++\<^bsub>S\<^esub> m2 f! x = m2 f! x"
-  by (transfer, auto)
+  by (auto simp add: fmap_add_def lookup_def fdom_def)
 
 lemma lookup_fmap_add2[simp]:  "x \<notin> S \<Longrightarrow>  m1 f++\<^bsub>S\<^esub> m2 f! x = m1 f! x"
-  by (transfer, simp)
+  by (auto simp add: fmap_add_def lookup_def fdom_def)
 
 lemma lookup_fmap_add_eq: " m1 f++\<^bsub>S\<^esub> m2 f! x = (if x \<in> S then m2 f! x else m1 f! x)"
   by (cases "x \<notin> S") simp_all
 
-(*
-lemma fmap_add_overwrite: "fdom m1 \<subseteq> fdom m2 \<Longrightarrow> m1 f++ m2 = m2"
-  apply transfer
-  apply rule
-  apply (case_tac "x \<in> dom m2")
-  apply (auto simp add: map_add_dom_app_simps(1))
-  done
-*)
-
 lemma fmap_add_upd_swap: 
   "x \<notin> S \<Longrightarrow> \<rho>(x f\<mapsto> z) f++\<^bsub>S\<^esub> \<rho>' = (\<rho> f++\<^bsub>S\<^esub> \<rho>')(x f\<mapsto> z)"
-  by transfer auto
+  by (auto simp add: fmap_add_def fmap_upd_def lookup_def fdom_def)
 
 lemma fmap_add_upd: 
   "x \<in> S \<Longrightarrow> \<rho> f++\<^bsub>S\<^esub> (\<rho>'(x f\<mapsto> z)) = (\<rho> f++\<^bsub>S - {x}\<^esub> \<rho>')(x f\<mapsto> z)"
-  apply transfer
-  apply rule
-  apply auto
-  done
+  by (auto simp add: fmap_add_def fmap_upd_def lookup_def fdom_def)
 
 lemma fmap_restr_add: "fmap_restr S (m1 f++\<^bsub>S2\<^esub> m2) = fmap_restr S m1 f++\<^bsub>S2\<^esub> fmap_restr S m2"
-  apply (rule fmap_eqI)
-  apply (case_tac "x \<in> S2")
-  apply (case_tac [!] "x \<in> S")
-  apply auto
-  done
+  by (auto simp add: fmap_add_def fmap_upd_def lookup_def fdom_def fmap_restr_def)
 
 lemma fmap_delete_add: "fmap_delete x (m1 f++\<^bsub>S\<^esub> m2) = fmap_delete x m1 f++\<^bsub>S - {x}\<^esub> fmap_delete x m2"
-  apply (rule fmap_eqI)
-  apply (case_tac "xa = x")
-  apply (case_tac [!] "xa \<in> S")
-  apply auto
-  done
+  by (auto simp add: fmap_add_def fmap_upd_def lookup_def fdom_def fmap_restr_def fmap_delete_def)
 
+(*
 subsubsection {* Copying *}
 
 lift_definition fmap_copy :: "'a f\<rightharpoonup> 'b \<Rightarrow> 'a \<Rightarrow> 'a \<Rightarrow> 'a f\<rightharpoonup> 'b"
@@ -261,27 +230,26 @@ lemma fmap_restrict_fmap_copy[simp]: "x \<notin> S \<Longrightarrow> fmap_restr 
 
 lemma fmap_restrict_fmap_copy'[simp]: "x \<in> S \<Longrightarrow> y \<in> S \<Longrightarrow> fmap_restr S (fmap_copy \<Gamma> y x) = fmap_copy (fmap_restr S \<Gamma>) y x"
   by transfer auto
+*)
+
 
 subsubsection {* Map *}
 
-lift_definition fmap_map :: "('b \<Rightarrow> 'c) \<Rightarrow> 'a f\<rightharpoonup> 'b \<Rightarrow> 'a f\<rightharpoonup> 'c" is "\<lambda> f m x. f (m x)"..
+definition fmap_map :: "('b \<Rightarrow> 'c) \<Rightarrow> 'a f\<rightharpoonup> 'b \<Rightarrow> 'a f\<rightharpoonup> 'c" where "fmap_map f m = (\<lambda> x. f (m x))"
 
-lemma fmap_map_id[simp]: "fmap_map (\<lambda> x. x) m = m" by transfer (simp add: Option.map.identity)
+lemma fmap_map_id[simp]: "fmap_map (\<lambda> x. x) m = m" by (simp add: fmap_map_def)
 
-(*
-lemma fdom_fmap_map[simp]: "fdom (fmap_map f m) = fdom m" by transfer (simp add: dom_def)
-*)
-
-lemma lookup_fmap_map[simp]: "lookup (fmap_map f m) x = f (lookup m x)" by transfer simp
+lemma lookup_fmap_map[simp]: "lookup (fmap_map f m) x = f (lookup m x)"  by (simp add: fmap_map_def lookup_def)
 
 lemma fmap_map_fmap_restr[simp]: "f \<bottom> = \<bottom> \<Longrightarrow> fmap_map f (fmap_restr S m) = fmap_restr S (fmap_map f m)"
   by (rule fmap_eqI) (auto simp add: lookup_fmap_restr_eq)
 
 lemma fmap_map_fmap_upd[simp]: "fmap_map f (m(x f\<mapsto> v)) = (fmap_map f m)(x f\<mapsto> f v)"
-  by transfer auto
-
+  by (auto simp add: fmap_map_def lookup_def fmap_upd_def)
+(*
 lemma fmap_map_fmap_copy [simp]: "fmap_map f (fmap_copy m x y) = fmap_copy (fmap_map f m) x y"
   by transfer auto
+*)
 
 (*
 subsubsection {* Conversion from associative lists *}
