Launchbury/Denotational.thy
@@ -6,7 +6,7 @@ interpretation semantic_domain Fn Fn_project "\<Lambda> x. x".
 
 abbreviation ESem_syn'' ("\<lbrakk> _ \<rbrakk>\<^bsub>_\<^esub>"  [60,60] 60) where "\<lbrakk> e \<rbrakk>\<^bsub>\<rho>\<^esub> \<equiv> ESem e \<cdot> \<rho>"
 abbreviation HSem_syn' ("\<lbrace>_\<rbrace>_"  [60,60] 60) where "\<lbrace>\<Gamma>\<rbrace>\<rho> \<equiv> HSem \<Gamma> \<cdot> \<rho>"
-abbreviation HSem_fempty  ("\<lbrace>_\<rbrace>"  [60] 60) where "\<lbrace>\<Gamma>\<rbrace> \<equiv> \<lbrace>\<Gamma>\<rbrace>f\<emptyset>"
+abbreviation HSem_fempty  ("\<lbrace>_\<rbrace>"  [60] 60) where "\<lbrace>\<Gamma>\<rbrace> \<equiv> \<lbrace>\<Gamma>\<rbrace>\<bottom>"
 
 
 subsubsection {* Replacing subexpressions by variables *}
