Launchbury/Env-Nominal.thy
@@ -2,45 +2,21 @@ theory "Env-Nominal"
   imports Env "Nominal-Utils" "Nominal-HOLCF"
 begin
 
-subsubsection {* Permtuations on finite maps *}
-
-instantiation "fmap" :: (pt,pcpo_pt) pt
-begin
-  lift_definition permute_fmap :: "perm \<Rightarrow> 'a f\<rightharpoonup> 'b \<Rightarrow> 'a f\<rightharpoonup> 'b"
-    is "\<lambda> p f . p \<bullet> f" ..
-  
-  instance
-  apply(default)
-  apply(transfer, simp)+
-  done
-end
-
 subsubsection {* Equivariance lemmas related to finite maps *}
 
 lemma lookup_eqvt[eqvt]:
   "\<pi> \<bullet> lookup m x = lookup (\<pi> \<bullet> m) (\<pi> \<bullet> x)"
-  by transfer simp
+  by (simp add: lookup_def)
 
 lemma the_lookup_perm[simp]:
   fixes \<rho> :: "'a::at_base f\<rightharpoonup> 'b::{pure,pcpo_pt}"
   shows "((x' \<leftrightarrow> x) \<bullet> \<rho>) f! xa = \<rho> f! ((x' \<leftrightarrow> x) \<bullet> xa) " 
   by (metis lookup_eqvt permute_flip_cancel permute_pure)
 
-lemma fempty_eqvt[eqvt, simp]:
-  "\<pi> \<bullet> f\<emptyset> = f\<emptyset>"
-  by transfer auto
-
-lemma fempty_supp[simp]: "supp f\<emptyset> = {}"
-  by (metis eqvt_def fempty_eqvt supp_fun_eqvt)
-
-lemma fempty_fresh[simp]: "a \<sharp> f\<emptyset>"
-  by (simp add: fresh_def)
-
-lemma fempty_fresh_star[simp]: "a \<sharp>* f\<emptyset>"
-  by (simp add: fresh_star_def)
-
-lemma fdom_perm: "fdom (\<pi> \<bullet> f) = \<pi> \<bullet> (fdom f)"
-  by transfer auto
+lemma fdom_perm:
+  fixes f :: "'a::pt f\<rightharpoonup> 'b::{pcpo_pt}"
+  shows "fdom (\<pi> \<bullet> f) = \<pi> \<bullet> (fdom f)"
+  by (simp add: fdom_def)
 
 lemmas fdom_perm_rev[simp,eqvt] = fdom_perm[symmetric]
 
@@ -50,23 +26,28 @@ lemma mem_fdom_perm[simp]:
   by (metis (mono_tags) fdom_perm_rev mem_Collect_eq permute_set_eq)
 
 lemma fmap_upd_eqvt[eqvt]: "p \<bullet> (fmap_upd f x y) = fmap_upd (p \<bullet> f) (p \<bullet> x) (p \<bullet> y)"
-  by transfer (metis fun_upd_eqvt)
+  by (simp add: fmap_upd_def fun_upd_eqvt)
 
 lemma fmap_restr_eqvt[eqvt]:
-  "\<pi> \<bullet> m f|` d = (\<pi> \<bullet> m) f|` (\<pi> \<bullet> d)"
-  by transfer auto
+  fixes m :: "'a::pt f\<rightharpoonup> 'b::{cont_pt,pcpo}"
+  shows "\<pi> \<bullet> m f|` d = (\<pi> \<bullet> m) f|` (\<pi> \<bullet> d)"
+  by (auto simp add: fmap_restr_def lookup_def )
 
 lemma fmap_delete_eqvt[eqvt]:
-  "\<pi> \<bullet> fmap_delete x m = fmap_delete (\<pi> \<bullet> x) (\<pi> \<bullet> m)"
-  by transfer simp
+  fixes m :: "'a::pt f\<rightharpoonup> 'b::{cont_pt,pcpo}"
+  shows "\<pi> \<bullet> fmap_delete x m = fmap_delete (\<pi> \<bullet> x) (\<pi> \<bullet> m)"
+  by (auto simp add: fmap_delete_def lookup_def )
 
+(*
 lemma fmap_copy_eqvt[eqvt]:
   "\<pi> \<bullet> fmap_copy m a b = fmap_copy (\<pi> \<bullet> m) (\<pi> \<bullet> a) (\<pi> \<bullet> b)"
   by transfer simp
+*)
 
 lemma fmap_add_eqvt[eqvt]:
-  "\<pi> \<bullet> m1 f++\<^bsub>S\<^esub> m2 = (\<pi> \<bullet> m1) f++\<^bsub>\<pi> \<bullet> S\<^esub> (\<pi> \<bullet> m2)"
-  by transfer simp
+  fixes m1 m2 :: "'a::pt f\<rightharpoonup> 'b::{cont_pt,pcpo}"
+  shows "\<pi> \<bullet> m1 f++\<^bsub>S\<^esub> m2 = (\<pi> \<bullet> m1) f++\<^bsub>\<pi> \<bullet> S\<^esub> (\<pi> \<bullet> m2)"
+  by (auto simp add: fmap_add_def lookup_def )
 
 (*
 lemma fmap_of_eqvt[eqvt]:
@@ -74,9 +55,11 @@ lemma fmap_of_eqvt[eqvt]:
   by transfer (rule map_of_eqvt)
 *)
 
+(*
 lemma fmap_map_eqvt[eqvt]:
   "\<pi> \<bullet> fmap_map f m = fmap_map (\<pi> \<bullet> f) (\<pi> \<bullet> m)"
 by transfer simp
+*)
 
 subsubsection {* Permutation and restriction *}
 
@@ -85,12 +68,12 @@ lemma fmap_restr_perm:
   assumes "supp p \<sharp>* S" and [simp]: "finite S"
   shows "(p \<bullet> \<rho>) f|` S = \<rho> f|` S"
 using assms
-apply transfer
-apply rule
+apply -
+apply (rule fmap_eqI)
 apply (case_tac "x \<in> S")
 apply (simp)
 apply (subst permute_fun_def)
-apply (simp add: permute_pure)
+apply (simp add: permute_pure lookup_def)
 apply (subst perm_supp_eq)
 apply (auto simp add:perm_supp_eq supp_minus_perm fresh_star_def fresh_def supp_set_elem_finite)
 done
@@ -100,9 +83,9 @@ lemma fmap_restr_flip:
   assumes "x \<notin> S" and "x' \<notin> S"
   shows "((x' \<leftrightarrow> x) \<bullet> \<rho>) f|` S = \<rho> f|` S"
   using assms
-  apply transfer
+  apply -
   apply rule
-  apply (auto  simp add: permute_flip_at split:if_splits)
+  apply (auto  simp add: permute_flip_at lookup_def fmap_restr_def split:if_splits)
   by (metis eqvt_lambda flip_at_base_simps(3) minus_flip permute_pure unpermute_def)
 
 end
