Launchbury/HOLCF-Utils.thy
@@ -2,4 +2,33 @@ theory "HOLCF-Utils"
   imports HOLCF
 begin
 
+default_sort type
+
+lemma cont_compose2:
+  assumes "cont c"
+  assumes "\<And> x. cont (c x)"
+  assumes "cont f"
+  assumes "cont g"
+  shows "cont (\<lambda>x. c (f x) (g x))"
+proof-
+  have "monofun (\<lambda>x. c (f x) (g x))"
+    apply (rule monofunI)
+    apply (rule below_trans[OF cont2monofunE[OF assms(2) cont2monofunE[OF `cont g`]]], assumption)
+    apply (rule fun_belowD[OF cont2monofunE[OF `cont c` cont2monofunE[OF `cont f`]]], assumption)
+    done
+  thus ?thesis
+    apply (rule contI2)
+    apply (subst cont2contlubE[OF `cont f`], assumption)
+    apply (subst cont2contlubE[OF `cont g`], assumption)
+    apply (subst cont2contlubE[OF `cont c` ch2ch_cont[OF `cont f`]], assumption)
+    apply (subst lub_fun[OF ch2ch_cont[OF `cont c` ch2ch_cont[OF `cont f`]]], assumption)
+    apply (subst cont2contlubE[OF assms(2)ch2ch_cont[OF `cont g`]], assumption)
+    apply (subst diag_lub)
+    apply (rule ch2ch_fun[OF ch2ch_cont[OF `cont c` ch2ch_cont[OF `cont f`]]], assumption)
+    apply (rule ch2ch_cont[OF assms(2) ch2ch_cont[OF `cont g`]], assumption)
+    apply (rule below_refl)
+    done
+qed
+
+
 end
