Launchbury/ResourcedDenotational.thy
@@ -11,7 +11,7 @@ interpretation semantic_domain
 
 abbreviation ESem_syn'' ("\<N>\<lbrakk> _ \<rbrakk>\<^bsub>_\<^esub>"  [60,60] 60) where "\<N>\<lbrakk> e \<rbrakk>\<^bsub>\<rho>\<^esub> \<equiv> ESem e \<cdot> \<rho>"
 abbreviation HSem_syn' ("\<N>\<lbrace>_\<rbrace>_"  [60,60] 60) where "\<N>\<lbrace>\<Gamma>\<rbrace>\<rho> \<equiv> HSem \<Gamma> \<cdot> \<rho>"
-abbreviation HSem_fempty  ("\<N>\<lbrace>_\<rbrace>"  [60] 60) where "\<N>\<lbrace>\<Gamma>\<rbrace> \<equiv> \<N>\<lbrace>\<Gamma>\<rbrace>fempty"
+abbreviation HSem_fempty  ("\<N>\<lbrace>_\<rbrace>"  [60] 60) where "\<N>\<lbrace>\<Gamma>\<rbrace> \<equiv> \<N>\<lbrace>\<Gamma>\<rbrace>\<bottom>"
 
 (* The same, but with some beta_cfun's and eta_cfuns resolved.*)
 lemma CESem_simps:
